Towards subject reduction
Proving valid_btys: needs more inversion info on |- tInd args : tau
Add Derive Signature where needed to avoid warnings
Proved inversion lemmas on typing spine
Finished inversion of |- c : mkApps (tInd ind u) args, remain some holes in valid_btys
related to universes and the typing of the branches.

One todo + 2 universes properties

WIP valid_btys

state elim restriction
Backport of cdacc4de201

WIP proving inversion of constructor typing by inductive (provable!)

Finish Construct_Ind_ind_eq

Modify type_local_ctx so that it implies wf_local_env (adding proofs for lets)

Prove a strong subst lemma for typing_spines of it_mkProd_or_LetIn

WIP

Prove substitutivity of `isType (it_mkProd_or_LetIn)`

WIP proving valid_btys

WIP subslet_app_inv proof

WIP rebsing valid_btys and cleaning up

WIP refactoring

Move more defs to the Env and inline them

Fix erasure

Fix proof focusing in PCUIC

Refactor. The remaining safe lemmata all require SR

WIP proving SR for Case

WIP on SR proof

WIP finishing SR proof

WIP proving SR

WIP proving SR for match

Fix after rebase

Force no output of examples due to timing files

Fix after rebase

template-coq/theories/EnvironmentTyping.v
@@ -253,23 +253,24 @@ Module DeclarationTyping (T : Term) (E : EnvironmentSig T)
     Context (P : global_env_ext -> context -> term -> option term -> Type).
 
     (** For well-formedness of inductive declarations we need a way to check that a assumptions
-        of a given context is typable in a sort [u]. *)
-    Fixpoint type_local_ctx Σ (Γ Δ : context) (u : Universe.t) : Type :=
+      of a given context is typable in a sort [u]. We also force well-typing of the let-ins
+      in any universe to imply wf_local. *)
+      Fixpoint type_local_ctx Σ (Γ Δ : context) (u : Universe.t) : Type :=
       match Δ with
       | [] => True
-      | {| decl_body := None ; decl_type := t |} :: Δ =>
-        (type_local_ctx Σ Γ Δ u * (P Σ (Γ ,,, Δ) t (Some (tSort u))))
-      | {| decl_body := Some _ |} :: Δ =>
-        type_local_ctx Σ Γ Δ u
-      end.
+      | {| decl_body := None; decl_type := t |} :: Δ => (type_local_ctx Σ Γ Δ u * (P Σ (Γ ,,, Δ) t (Some (tSort u))))
+      | {| decl_body := Some b; decl_type := t |} :: Δ => (type_local_ctx Σ Γ Δ u * (P Σ (Γ ,,, Δ) t None * P Σ (Γ ,,, Δ) b (Some t)))
+      end.    
 
     Implicit Types (mdecl : mutual_inductive_body) (idecl : one_inductive_body) (cdecl : ident * term * nat).
 
     Definition on_type Σ Γ T := P Σ Γ T None.
 
-    Record constructor_shape mdecl i idecl ctype :=
+    Record constructor_shape mdecl i idecl ctype cargs :=
       { cshape_args : context;
         (* Arguments (with lets) *)
+        cshape_args_length : context_assumptions cshape_args = cargs;
+        (* Real (non-let) arguments bound by the constructor *)
 
         cshape_concl_head := tRel (#|mdecl.(ind_bodies)|
                                   - S i
@@ -290,17 +291,17 @@ Module DeclarationTyping (T : Term) (E : EnvironmentSig T)
           arguments ending with a reference to the inductive applied to the
           (non-lets) parameters and arguments *)
       }.
-    Arguments cshape_args {mdecl i idecl ctype}.
+    Arguments cshape_args {mdecl i idecl ctype cargs}.
 
     Open Scope type_scope.
 
     Definition on_constructor Σ mdecl i idecl cdecl ind_ctor_sort :=
       (* cdecl.1 fresh ?? *)
-      (* cdecl.2.2 ?? *)
       let ctype := cdecl.1.2 in
+      let cargs := cdecl.2 in
       (* FIXME: there is some redundancy with the type_local_ctx *)
       on_type Σ (arities_context mdecl.(ind_bodies)) ctype *
-      { cs : constructor_shape mdecl i idecl ctype &
+      { cs : constructor_shape mdecl i idecl ctype cargs &
             type_local_ctx Σ
                       (arities_context mdecl.(ind_bodies) ,,, mdecl.(ind_params))
                       cs.(cshape_args) ind_ctor_sort }.
@@ -475,7 +476,7 @@ Module DeclarationTyping (T : Term) (E : EnvironmentSig T)
 
   End GlobalMaps.
 
-  Arguments cshape_args {mdecl i idecl ctype}.
+  Arguments cshape_args {mdecl i idecl ctype cargs}.
   Arguments ind_indices {_ P Σ mind mdecl i idecl}.
   Arguments ind_sort {_ P Σ mind mdecl i idecl}.
   Arguments ind_arity_eq {_ P Σ mind mdecl i idecl}.
@@ -512,7 +513,7 @@ Module DeclarationTyping (T : Term) (E : EnvironmentSig T)
   Proof.
     intros HP HPQ. revert HP; induction Δ in Γ, HPQ |- *; simpl; auto.
     destruct a as [na [b|] ty]; simpl; auto.
-    intros. intuition auto.
+    intros. intuition auto. intuition auto.
   Qed.
 
   (** This predicate enforces that there exists typing derivations for every typable term in env. *)
