checker/theories/Closed.v
@@ -2,7 +2,7 @@
 
 From Coq Require Import Bool List Program ZArith Lia.
 From MetaCoq.Template Require Import config utils Ast AstUtils Induction
-  LiftSubst UnivSubst Typing.
+  LiftSubst UnivSubst Typing TypingWf.
 From MetaCoq.Checker Require Import WeakeningEnv.
 Require Import ssreflect.
 
@@ -377,52 +377,6 @@ Proof.
       move/andP: Hwfi => [] clΓ clctx.
       apply closedn_it_mkProd_or_LetIn => //.
     + destruct s. rewrite andb_true_r in p. intuition auto.
-Qed.
-
-Lemma on_global_env_impl `{checker_flags} Σ P Q :
-  (forall Σ Γ t T, on_global_env P Σ.1 -> P Σ Γ t T -> Q Σ Γ t T) ->
-  on_global_env P Σ -> on_global_env Q Σ.
-Proof.
-  intros X X0.
-  simpl in *. induction X0; constructor; auto.
-  clear IHX0. destruct d; simpl.
-  - destruct c; simpl. destruct cst_body; simpl in *.
-    red in o |- *. simpl in *. now eapply X.
-    red in o |- *. simpl in *. now eapply X.
-  - red in o. simpl in *.
-    destruct o0 as [onI onP onNP].
-    constructor; auto.
-    -- eapply Alli_impl. exact onI. eauto. intros.
-       refine {| ind_indices := X1.(ind_indices);
-                 ind_arity_eq := X1.(ind_arity_eq);
-                 ind_ctors_sort := X1.(ind_ctors_sort) |}.
-       --- apply onArity in X1. unfold on_type in *; simpl in *.
-           now eapply X.
-       --- pose proof X1.(onConstructors) as X11. red in X11.
-           unfold on_constructor, on_type in *. eapply All2_impl; eauto.
-           simpl. intros. destruct X2 as (? & ? & ?).
-           split. now eapply X.
-           exists x1.
-           clear -t X X0.
-           revert t. generalize (cshape_args x1).
-           abstract (induction c; simpl; auto;
-           destruct a as [na [b|] ty]; simpl in *; auto;
-           split; eauto; [apply IHc;apply t|apply X;simpl; auto;apply t]).
-       --- simpl; intros. pose (onProjections X1 H0). simpl in *.
-           destruct o0. constructor; auto. eapply Alli_impl; intuition eauto.
-           unfold on_projection in *; simpl in *.
-           now apply X.
-       --- destruct X1. simpl. unfold check_ind_sorts in *.
-           destruct universe_family; auto.
-           split. apply ind_sorts. destruct indices_matter; auto.
-           eapply type_local_ctx_impl. eapply ind_sorts. auto.
-           split; [apply fst in ind_sorts|apply snd in ind_sorts].
-           eapply Forall_impl; tea. auto.
-           destruct indices_matter; [|trivial].
-           eapply type_local_ctx_impl; tea. eauto.
-    -- red in onP. red.
-       eapply All_local_env_impl. eauto.
-       intros. now apply X.
 Qed.
 
 
